fix: rewrite sllb; add some lemmas

TheoryTask/qcp-binary-democases/SeparationLogic/examples/sll_project_lib.v
@@ -59,14 +59,329 @@ Fixpoint sllbseg (x y: addr) (l: list Z): Assertion :=
    - head: pointer to the first node (or NULL if empty)
    - ptail: pointer to the 'next' field of the last node (or &head if empty)
    
-   Note: This predicate does NOT include the *ptail permission because
-   sll already contains the last node's next field (which equals NULL).
-   Functions that need to modify *ptail must use expanded specifications.
+   New design using sllbseg to properly track *ptail permission:
+   - Empty list: head = NULL, ptail = &head
+   - Non-empty list: sllbseg from &head to ptail, and *ptail = NULL
 *)
 Definition sllb (x: addr) (l: list Z): Assertion :=
+  [| x <> NULL |] &&
+  EX ptail_val: addr,
+    &(x # "sllb" ->ₛ "ptail") # Ptr |-> ptail_val **
+    sllbseg (&(x # "sllb" ->ₛ "head")) ptail_val l **
+    ptail_val # Ptr |-> NULL.
+
+(* ============================================================ *)
+(* Auxiliary lemmas for sll (adapted from sll_lib.v) *)
+(* ============================================================ *)
+
+Lemma sll_zero: forall x l,
+  x = NULL ->
+  sll x l |-- [| l = nil |] && emp.
+Proof.
+  intros.
+  destruct l.
+  + entailer!.
+  + simpl.
+    Intros. Intros x0.
+    entailer!.
+Qed.
+
+Lemma sll_not_zero: forall x l,
+  x <> NULL ->
+  sll x l |--
+    EX y a l0,
+      [| l = a :: l0 |] &&
+      &(x # "sll" ->ₛ "data") # Int |-> a **
+      &(x # "sll" ->ₛ "next") # Ptr |-> y **
+      sll y l0.
+Proof.
+  intros.
+  destruct l.
+  + simpl.
+    Intros.
+    tauto.
+  + simpl. Intros.
+    Intros y.
+    Exists y z l.
+    entailer!.
+Qed.
+
+Lemma sll_not_zero': forall x l,
+  x <> NULL ->
+  sll x l |-- [| l <> nil |].
+Proof.
+  intros.
+  destruct l.
+  + simpl.
+    Intros.
+    tauto.
+  + simpl. Intros.
+    Intros y.
+    entailer!.
+    congruence.
+Qed.
+
+Lemma sllseg_len1: forall x a y,
+  x <> NULL ->
+  &(x # "sll" ->ₛ "data") # Int |-> a **
+  &(x # "sll" ->ₛ "next") # Ptr |-> y |--
+  sllseg x y [a].
+Proof.
+  intros.
+  simpl sllseg.
+  Exists y.
+  entailer!.
+Qed.
+
+Lemma sllseg_sllseg: forall x y z l1 l2,
+  sllseg x y l1 ** sllseg y z l2 |--
+  sllseg x z (l1 ++ l2).
+Proof.
+  intros.
+  revert x; induction l1; simpl sllseg; intros.
+  + Intros.
+    subst y.
+    entailer!.
+  + Intros. Intros z0.
+    Exists z0.
+    sep_apply IHl1.
+    entailer!.
+Qed.
+
+Lemma sllseg_sll: forall x y l1 l2,
+  sllseg x y l1 ** sll y l2 |--
+  sll x (l1 ++ l2).
+Proof.
+  intros.
+  revert x; induction l1; simpl sllseg; simpl sll; intros.
+  + Intros.
+    subst y.
+    entailer!.
+  + Intros. Intros z0.
+    Exists z0.
+    sep_apply IHl1.
+    entailer!.
+Qed.
+
+Lemma sllbseg_2_sllseg: forall x y z l,
+  sllbseg x y l ** y # Ptr |-> z |--
+  EX y': addr, x # Ptr |-> y' ** sllseg y' z l.
+Proof.
+  intros.
+  revert x; induction l; simpl; intros.
+  + Intros.
+    subst x.
+    Exists z; entailer!.
+  + Intros x_v.
+    Exists x_v.
+    sep_apply IHl.
+    Intros y'.
+    Exists y'.
+    entailer!.
+Qed.
+
+Lemma sllbseg_len1: forall (x y: addr) (a: Z),
+  y <> 0 ->
+  x # Ptr |-> y **
+  &( y # "sll" ->ₛ "data") # Int |-> a |--
+  sllbseg x (&( y # "sll" ->ₛ "next")) [a].
+Proof.
+  intros.
+  simpl.
+  Exists y.
+  entailer!.
+Qed.
+
+Lemma sllbseg_sllbseg: forall x y z l1 l2,
+  sllbseg x y l1 ** sllbseg y z l2 |--
+  sllbseg x z (l1 ++ l2).
+Proof.
+  intros.
+  revert x; induction l1; simpl; intros.
+  + entailer!.
+    subst x.
+    entailer!.
+  + Intros u.
+    Exists u.
+    entailer!.
+Qed.
+
+Lemma sllseg_0_sll: forall x l,
+  sllseg x 0 l |-- sll x l.
+Proof.
+  intros. revert x. 
+  induction l; try easy.
+  simpl. intros. 
+  Intros z. Exists z. entailer!.
+Qed.
+
+(* ============================================================ *)
+(* Lemmas for map_mult *)
+(* ============================================================ *)
+
+Lemma map_mult_nil: forall x,
+  map_mult x nil = nil.
+Proof.
+  reflexivity.
+Qed.
+
+Lemma map_mult_cons: forall x a l,
+  map_mult x (a :: l) = (x * a) :: map_mult x l.
+Proof.
+  reflexivity.
+Qed.
+
+(* ============================================================ *)
+(* Lemmas for sllb *)
+(* ============================================================ *)
+
+(* sllb with nil list: head = NULL, ptail = &head *)
+Lemma sllb_zero: forall x,
+  sllb x nil |--
+  [| x <> NULL |] &&
+  &(x # "sllb" ->ₛ "head") # Ptr |-> NULL **
+  &(x # "sllb" ->ₛ "ptail") # Ptr |-> &(x # "sllb" ->ₛ "head").
+Proof.
+  intros.
+  unfold sllb.
+  Intros ptail_val.
+  simpl sllbseg.
+  Intros.
+  subst ptail_val.
+  entailer!.
+Qed.
+
+(* sllb with non-empty list: expose first node *)
+Lemma sllb_not_zero: forall x a l,
+  sllb x (a :: l) |--
+  EX head_val ptail_val: addr,
+    [| x <> NULL |] &&
+    [| head_val <> NULL |] &&
+    &(x # "sllb" ->ₛ "head") # Ptr |-> head_val **
+    &(x # "sllb" ->ₛ "ptail") # Ptr |-> ptail_val **
+    &(head_val # "sll" ->ₛ "data") # Int |-> a **
+    sllbseg (&(head_val # "sll" ->ₛ "next")) ptail_val l **
+    ptail_val # Ptr |-> NULL.
+Proof.
+  intros.
+  unfold sllb.
+  Intros ptail_val.
+  simpl sllbseg.
+  Intros head_val.
+  Exists head_val ptail_val.
+  entailer!.
+Qed.
+
+(* sllb len1: construct sllb with single element *)
+Lemma sllb_len1: forall x,
+  x <> NULL ->
+  &(x # "sllb" ->ₛ "head") # Ptr |-> NULL **
+  &(x # "sllb" ->ₛ "ptail") # Ptr |-> &(x # "sllb" ->ₛ "head") |--
+  sllb x nil.
+Proof.
+  intros.
+  unfold sllb.
+  Exists (&(x # "sllb" ->ₛ "head")).
+  simpl sllbseg.
+  entailer!.
+Qed.
+
+(* sllb_2_sllbseg: convert sllb to sllbseg + *ptail = 0 *)
+Lemma sllb_2_sllbseg: forall x l,
+  sllb x l |--
+  EX ptail_val: addr,
+    [| x <> NULL |] &&
+    &(x # "sllb" ->ₛ "ptail") # Ptr |-> ptail_val **
+    sllbseg (&(x # "sllb" ->ₛ "head")) ptail_val l **
+    ptail_val # Ptr |-> NULL.
+Proof.
+  intros.
+  unfold sllb.
+  Intros ptail_val.
+  Exists ptail_val.
+  entailer!.
+Qed.
+
+(* sllbseg_0_sll: convert sllbseg + *ptail = 0 to sll *)
+Lemma sllbseg_0_sll': forall x y l,
+  sllbseg x y l ** y # Ptr |-> NULL |--
+  EX head_val: addr, x # Ptr |-> head_val ** sll head_val l.
+Proof.
+  intros.
+  revert x; induction l; simpl; intros.
+  + Intros.
+    subst x.
+    Exists NULL.
+    simpl sll.
+    entailer!.
+  + Intros head_val.
+    Exists head_val.
+    sep_apply IHl.
+    Intros next_val.
+    simpl sll.
+    Exists next_val.
+    entailer!.
+Qed.
+
+(* sllb_2_sll: convert sllb to sll representation *)
+Lemma sllb_2_sll: forall x l,
+  sllb x l |--
   EX head_val ptail_val: addr,
     [| x <> NULL |] &&
     &(x # "sllb" ->ₛ "head") # Ptr |-> head_val **
     &(x # "sllb" ->ₛ "ptail") # Ptr |-> ptail_val **
     sll head_val l.
+Proof.
+  intros.
+  unfold sllb.
+  Intros ptail_val.
+  sep_apply sllbseg_0_sll'.
+  Intros head_val.
+  Exists head_val ptail_val.
+  entailer!.
+Qed.
+
+(* sllbseg_2_sllb: construct sllb from sllbseg (reverse direction) *)
+Lemma sllbseg_2_sllb: forall x ptail_val l,
+  x <> NULL ->
+  &(x # "sllb" ->ₛ "ptail") # Ptr |-> ptail_val **
+  sllbseg (&(x # "sllb" ->ₛ "head")) ptail_val l **
+  ptail_val # Ptr |-> NULL |--
+  sllb x l.
+Proof.
+  intros.
+  unfold sllb.
+  Exists ptail_val.
+  entailer!.
+Qed.
+
+(* sllbseg_sll: sllbseg + sll can form sll *)
+Lemma sllbseg_sll': forall x y l1 l2,
+  sllbseg x y l1 ** y # Ptr |-> 0 ** sll 0 l2 |--
+  EX h: addr, x # Ptr |-> h ** sll h (l1 ++ l2).
+Proof.
+  intros.
+  assert (H0: (0:addr) = NULL) by reflexivity.
+  sep_apply (sll_zero 0 l2 H0).
+  Intros.
+  subst l2.
+  rewrite app_nil_r.
+  sep_apply sllbseg_0_sll'.
+  Intros head_val.
+  Exists head_val.
+  entailer!.
+Qed.
+
+(* sllbseg_sll: sllbseg concatenation with sll *)
+Lemma sllbseg_sll: forall x y z l1 l2,
+  sllbseg x y l1 ** y # Ptr |-> z ** sll z l2 |--
+  EX h: addr, x # Ptr |-> h ** sll h (l1 ++ l2).
+Proof.
+  intros.
+  sep_apply sllbseg_2_sllseg.
+  Intros y'.
+  Exists y'.
+  sep_apply sllseg_sll.
+  entailer!.
+Qed.
 
