TheoryTask/qcp-binary-democases/SeparationLogic/examples/sll_project_goal.v
@@ -17,8 +17,8 @@ Local Open Scope list.
 Import naive_C_Rules.
 Require Import sll_project_lib.
 Local Open Scope sac.
-From SimpleC.EE Require Import common_strategy_goal.
-From SimpleC.EE Require Import common_strategy_proof.
+Require Import common_strategy_goal.
+Require Import common_strategy_proof.
 Require Import sll_project_strategy_goal.
 Require Import sll_project_strategy_proof.
 
